
\begin{align}
m_3(x_2) &= \sum_{x_3} P(X_3|X_2) P(X_4|X_3) \\
  &= \sum_{x_1} P(X_1 \cap X_2)\\
  &= P(X_2)\\
\implies \sum_{x_3} P(X_3|X_2) \sum_{x_4} P(X_4|X_3)\sum_{x_1} P(X_1)P(X_2|X_1) &= \sum_{x_3} P(X_3|X_2) m_1(x_2) \sum_{x_4} P(X_4|X_3)
\end{align}

\begin{align}
m_4(x_3) &= \sum_{x_4} P(X_4|X_3)\\
  &= 1\\
\implies \sum_{x_3} P(X_3|X_2) m_1(x_2) \sum_{x_4} P(X_4|X_3) &= \sum_{x_3} P(X_3|X_2) m_1(x_2)
\end{align}

\begin{align}
m_3(x_2) &= \sum_{x_3} P(X_3|X_2) m_1(X_2)\\
  &= \sum_{x_3} P(X_3|X_2) P(X_2)\\
  &= \sum_{x_3} P(X_3 \cap X_2)\\
  &= P(X_2)
\end{align}
